

$$1) \quad 2) \quad \left(\frac{a}{r}\right)^3 \sin 2v \quad \text{---} = x$$

$$\bar{x} = \frac{1}{2\pi} \int_0^{2\pi} \left(\frac{a}{r}\right)^3 \sin v \, dM$$

$$= \frac{1}{2\pi} \int_0^{2\pi} \left(\frac{a}{r}\right)^3 \sin v \frac{r^2}{a^2 \sqrt{1-e^2}} \, dv$$

$$= \frac{1}{2\pi} \cdot \frac{a}{\sqrt{1-e^2}} \int_0^{2\pi} \frac{\sin 2v}{r} \, dv$$

$$= \frac{a}{2\pi(1-e^2)\sqrt{1-e^2}} \int_0^{2\pi} \sin 2v \cdot (1+e\cos v) \, dv$$

$$= \int_0^{2\pi} \sin 2v \, dv + e \int_0^{2\pi} \cos v \sin 2v \, dv$$

$$= 0 = \left(\frac{a}{r}\right)^3 \sin 2v$$

$$1) \quad 2) \quad \left(\frac{a}{r}\right)^4 \cos v$$

$$\overline{\left(\frac{a}{r}\right)^4 \cos v} = \frac{1}{2\pi} \int_0^{2\pi} \left(\frac{a}{r}\right)^4 \cos v \, dM$$

$$= \frac{a^2}{2\pi \sqrt{1-e^2}} \int_0^{2\pi} r^2 \cos v \, dv$$

$$= \frac{a^2}{\underbrace{2\pi \sqrt{1-e^2} \cdot a^2 (1-e^2)^2}} \int_0^{2\pi} \cos v (1+e \cos v)^2 \, dv$$

$$= \frac{1}{2\pi \sqrt{1-e^2} (1-e^2)^2} \int_0^{2\pi} \cos v (1+2e \cos v + e^2 \cos^2 v) \, dv$$

$$= \frac{1}{2\pi \sqrt{1-e^2} (1-e^2)^2} \left(\int_0^{2\pi} \cos v \, dv + \int_0^{2\pi} \cos v \cdot 2e \cos v \, dv + \int_0^{2\pi} e^2 \cos^2 v \, dv \right)$$

\downarrow $\pi \cdot 2e$ \downarrow 0

$$= \frac{1}{2\pi \sqrt{1-e^2} (1-e^2)^2} \cdot 2e \cdot \pi = \boxed{\frac{e}{\sqrt{1-e^2} (1-e^2)^2} = \left(\frac{a}{r}\right)^4 \cos v}$$

1) 3) $\left(\frac{a}{r}\right)^5 \cos 2v$

$$\overline{\left(\frac{a}{r}\right)^5 \cos 2v} = \frac{1}{2\pi} \int_0^{2\pi} \left(\frac{a}{r}\right)^5 \cos 2v \, dv$$

~~scribbled out text~~

$$= \frac{1}{2\pi} \cdot \frac{a^2}{\sqrt{1-e^2}} \int_0^{2\pi} r^{-3} \cos 2v \, dv$$

$$= \frac{1}{2\pi} \cdot \frac{a^2}{\sqrt{1-e^2}} \cdot \frac{1}{a^2 (1-e^2)^3} \int_0^{2\pi} \cos 2v (1+e \cos v)^3 \, dv$$

$$= \frac{1}{2\pi \cdot \sqrt{1-e^2} \cdot (1-e^2)^3} \int_0^{2\pi} \cos 2v \cdot (1 + 3e \cos v + 3e^2 \cos^2 v + e^3 \cos^3 v) \, dv$$

$$= \frac{1}{2\pi \sqrt{1-e^2} \cdot (1-e^2)^3} \int_0^{2\pi} \cos 2v + 3e \cos v \cos 2v + 3e^2 \cos^2 v \cos 2v + e^3 \cos^3 v \cos 2v \, dv$$

$\frac{3\pi e^2}{2}$

$$= \frac{1}{2\pi \sqrt{1-e^2} (1-e^2)^3} \cdot \frac{3\pi e^2}{2} = \boxed{\frac{3e^2}{4\sqrt{1-e^2} (1-e^2)^3} \left(\frac{a}{r}\right)^5 \cos 2v}$$

$$2) \quad R \equiv \bar{R}_{sec} = -\frac{3}{2} \frac{n^2 R_\phi^2 J_2}{(1-e^2)^{3/2}} \left(\frac{\sin^2 i}{2} - \frac{1}{3} \right)$$

$$1) \quad \ddot{a}_{sec} = \frac{2}{na} \underbrace{\frac{\partial \bar{R}_{sec}}{\partial M_0}}_{\rightarrow 0} \quad \therefore \boxed{\ddot{a}_{sec} = 0}$$

$$2) \quad \dot{e}_{sec} = \frac{1-e^2}{na^2 e} \underbrace{\frac{\partial \bar{R}_{sec}}{\partial M_0}}_{\rightarrow 0} - \frac{\sqrt{1-e^2}}{na^2 e} \underbrace{\frac{\partial \bar{R}_{sec}}{\partial \omega}}_{\rightarrow 0}$$

$$\therefore \boxed{\dot{e}_{sec} = 0}$$

$$3) \quad \dot{i}_{sec} = \frac{1}{na^2 \sqrt{1-e^2} \sin i} \left(\cos i \cdot \underbrace{\frac{\partial \bar{R}_{sec}}{\partial \omega}}_{\rightarrow 0} - \underbrace{\frac{\partial \bar{R}_{sec}}{\partial \Omega}}_{\rightarrow 0} \right)$$

$$\therefore \boxed{\dot{i}_{sec} = 0}$$

$$4) \quad \dot{\omega}_{sec} = \frac{\sqrt{1-e^2}}{na^2 e} \frac{\partial \bar{R}_{sec}}{\partial e} - \frac{\cot i}{nc^2 \sqrt{1-e^2}} \frac{\partial \bar{R}_{sec}}{\partial i}$$

$$\begin{aligned} & \xrightarrow{\text{L}} -\frac{3}{2} \frac{n^2 R_\phi^2 J_2}{(1-e^2)^{3/2}} \left(\frac{\sin^2 i}{2} - \frac{1}{3} \right) \quad \xrightarrow{\text{L}} -\frac{3}{2} \frac{n^2 R_\phi^2 J_2}{(1-e^2)^{3/2}} \sin i \cos i \\ & \quad \frac{\sqrt{1-e^2}}{na^2 e} \cdot \frac{3}{2} \frac{n^2 R_\phi^2 J_2}{(1-e^2)^{3/2}} \left(\frac{\sin^2 i}{2} - \frac{1}{3} \right) - \frac{\cot i}{nc^2 \sqrt{1-e^2}} \cdot \frac{3}{2} \frac{n^2 R_\phi^2 J_2}{(1-e^2)^{3/2}} \sin i \cos i \\ & = \frac{3}{4} \frac{n R_\phi^2 J_2}{(1-e^2)^2} \left(-3 \sin^2 i + 2 + 2 \cos^2 i \right) \quad \xrightarrow{\text{L}} 2 - 2 \sin^2 i \\ & = \boxed{\frac{3 n R_\phi^2 J_2}{4 (1-e^2)^2} (-5 \sin^2 i + 4) = \dot{\omega}_{sec}} \end{aligned}$$

$$\begin{aligned}
 2) \quad 5) \quad \dot{M}_{0,sec} &= \frac{1-e^2}{na^2e} \frac{\partial \bar{R}_{sec}}{\partial e} - \frac{2}{na} \frac{\partial \bar{R}_{sec}}{\partial a} \\
 &\hookrightarrow -\frac{9}{2} \frac{n^2 R_\phi^2 T_2}{(1-e^2)^{5/2}} \left(\frac{\sin^2 i}{2} - \frac{1}{3} \right) \\
 &\quad \frac{-6n R_\phi^2 T_2}{(1-e^2)^{3/2}} \left(\frac{\sin^2 i}{2} - \frac{1}{3} \right) \left(-\frac{3}{2a} \right) \leftarrow \frac{\partial \bar{R}_{sec}}{\partial n} \cdot \frac{\partial n}{\partial a} \\
 &= \frac{9n R_\phi^2 T_2}{a(1-e^2)^{3/2}} \left(\frac{\sin^2 i}{2} - \frac{1}{3} \right)
 \end{aligned}$$

$$\begin{aligned}
 \dot{M}_{0,sec} &= \frac{1-e^2}{na^2e} \left(-\frac{9}{2} \frac{n^2 R_\phi^2 T_2}{(1-e^2)^{5/2}} \left(\frac{\sin^2 i}{2} - \frac{1}{3} \right) \right) \\
 &\quad - \frac{2}{na} \left(\frac{9n^2 R_\phi^2 T_2}{a(1-e^2)^{3/2}} \left(\frac{\sin^2 i}{2} - \frac{1}{3} \right) \right) \\
 &= -\frac{9}{2} \frac{n R_\phi^2 T_2}{a^2(1-e^2)^{3/2}} \left(\frac{\sin^2 i}{2} - \frac{1}{3} \right) - \frac{18n R_\phi^2 T_2}{a^2(1-e^2)^{3/2}} \left(\frac{\sin^2 i}{2} - \frac{1}{3} \right) \\
 &= \frac{n R_\phi^2 T_2}{a^2(1-e)^{3/2}} \left(-\frac{54}{2} (3\sin^2 i - 2) - 108 (3\sin^2 i - 2) \right) \\
 &= \cancel{-162} - \frac{135 n R_\phi^2 T_2}{a^2(1-e)^{3/2}} (3\sin^2 i - 2) = \dot{M}_{0,sec}
 \end{aligned}$$

$$3) \quad u_{4,0} = -T_4 \frac{\mu R_\phi^4}{8 r^5} (35 \sin^4 \phi - 30 \sin^2 \phi + 3)$$

$$\left(\frac{a}{r}\right)^5 = (1-e^2)^{-\frac{7}{2}} \left(1 + \frac{3}{2} e^2\right)$$

$$\begin{aligned} \sin^4 \phi &= \sin^4 i \sin^4(\omega + \nu) \\ &= \sin^4 i \left(\frac{3}{8} - \frac{1}{2} \cos 2(\omega + \nu) + \frac{1}{8} \cos 4(\omega + \nu) \right) \\ &= \frac{3}{8} \sin^4 i \end{aligned}$$

$$\begin{aligned} \sin^2 \phi &= \sin^2 i \sin^2(\omega + \nu) \\ &= \sin^2 i \left(\frac{1}{2} - \frac{1}{2} \cos 2(\omega + \nu) \right) \\ &= \frac{1}{2} \sin^2 i \end{aligned}$$

$$u_{4,0} = \frac{-T_4 \mu R_\phi^4}{8 r^5} \left(\frac{105}{8} \sin^4 i - 15 \sin^2 i + 3 \right)$$

$$\overline{u}_{4,0} = - \frac{T_4 \mu R_\phi^4}{8} \cdot \left(\frac{a^5}{r^5} \right) \cdot \frac{1}{a^5} \left(\frac{105 \sin^4 i}{8} - 15 \sin^2 i + 3 \right)$$

$$\begin{aligned} &= \frac{-T_4 \mu R_\phi^4}{8 a^5} \left(\frac{105 \sin^4 i}{8} - 15 \sin^2 i + 3 \right) \cdot (1-e^2)^{-7/2} \cdot \left(1 + \frac{3}{2} e^2 \right) \\ &= \overline{u}_{0,4} \end{aligned}$$

$$4) \dot{r}_{sec?} \quad \overline{u_{4,0}} = \frac{-T_4 \mu R_\oplus^4}{8a^5} \left(\frac{105 \sin^4 i}{8} - 15 \sin^2 i + 3 \right) (1-e^2)^{-7/2} \left(1 + \frac{3}{2} e^2 \right)$$

$$\dot{r}_{sec, T_4} = \frac{1}{a^2 (1-e^2)^{1/2} \sin i} \frac{\partial R_{sec, T_4}}{\partial i} \xrightarrow{\overline{u_{4,0}}} \downarrow \partial i$$

$$\frac{\partial R_{sec, T_4}}{\partial i} = \frac{-T_4 \mu R_\oplus^4}{8a^5} (1-e^2)^{-7/2} \left(1 + \frac{3}{2} e^2 \right) \cdot \left(\frac{105}{2} \sin^3 \cos i - 30 \sin i \cos i \right)$$

$$\dot{r}_{sec, T_4} = \frac{1}{a^2 (1-e^2)^{1/2} \sin i} \left(\frac{-T_4 \mu R_\oplus^4}{8a^5} (1-e^2)^{-7/2} \left(1 + \frac{3}{2} e^2 \right) \left(\frac{105}{2} \sin^2 \cos i - 30 \sin i \cos i \right) \right)$$

$$= \frac{1}{a^2 (1-e^2)^4} \cdot \frac{-T_4 \mu R_\oplus^4}{a^2} \left(1 + \frac{3}{2} e^2 \right) \left(\frac{105}{2} \sin^2 \cos i - 30 \sin i \cos i \right)$$

$$= \frac{-T_4 \mu R_\oplus^4}{a^4 (1-e^2)^4} \left(1 + \frac{3}{2} e^2 \right) 15 \cos i \left(\frac{7}{2} \sin^2 i - 2 \right)$$

$$= \boxed{\frac{-15 T_4 \mu R_\oplus^4 \cos i}{a^4 (1-e^2)^4} \left(1 + \frac{3}{2} e^2 \right) \left(\frac{7}{2} \sin^2 i - 2 \right)} = \dot{r}_{sec}$$

5)

$$r_p = 7200 \text{ km} \quad r_a = 7250 \text{ km} \quad i = 98^\circ$$

$$1) \dot{r}_{rel, J_2} = -\frac{3}{2} \cdot \frac{\sqrt{\mu} J_2 R_\oplus^2}{(1-e)^2 a^3} \cos i$$

$$2) \dot{r}_{sec, J_2} = \frac{-15 J_2 n R_\oplus^4 \cos i}{a^4 (1-e^2)^4} \left(1 + \frac{3}{4} e^2\right) \left(\frac{7}{2} \sin^2 i - 2\right)$$

3) J_2 is orders of magnitude larger & thus could lead to greater error.